\section{Homomorphism}

%%%%%%%%%%%%%%%
\begin{frame}{$D_6 \cong D_3 \times \mathbb{Z}_{2}$ (TJ 9.16)}
  \[
    D_6 = \set{1, r, r^2, r^3, r^4, r^5, s, rs, r^{2}s, r^{3}s, r^{4}s, r^{5}s}\; (r^6 = 1, s^2 = 1,
    srs = r^{-1})
  \]

  \[
    D_3 = \set{1, \rho, \rho^2, \lambda, \rho\lambda, \rho^{2}\lambda}\; (\rho^3 = 1, \lambda^2 = 1,
    \lambda\rho\lambda = \rho^{-1})
  \]

  \[
    \mathbb{Z}_{2} = \set{0, 1}
  \]

  \[
    f: D_6 \to D_3 \times \mathbb{Z}_{2}
  \]

  \[
    f: r \mapsto (\rho, 1), s \mapsto (\lambda, 1)
  \]

  \[
    D_8 \textcolor{gray}{\cong} D_4 \times \mathbb{Z}_{2}
  \]
\end{frame}
%%%%%%%%%%%%%%%
\begin{frame}{(TJ 9.16)}
  \[
    D_{2n} \cong D_{n} \times \mathbb{Z}_{2}\; (n \textrm{ is odd})
  \]

  \[
    f: r \mapsto (\rho, 1), s \mapsto (\lambda, 1)
  \]

  \[
    f: (r^{i}s^{j} \mapsto (\rho, 1)^{i} (\lambda, 1)^{j} = (\rho^{i}\lambda^{j}, 1^{i+j})\;
    (0 \le i < n, j \in \set{0,1})
  \]

  \[
    f((r^{i_1}s^{j_1})(r^{i_2}s^{j_2})) = (\rho^{i_1}\lambda^{j_1}, 1^{i_1 + j_1})
      (\rho^{i_2}\lambda^{j_2}, 1^{i_2 + j_2})
  \]

  \[
    f(r^{i_1}s^{j_1}r^{i_2}s^{j_2}) = (\rho^{i_1}\lambda^{j_1}\rho^{i_2}\lambda^{j_2}, 1^{i_1 + j_1
    + i_2 + j_2})
  \]

  \[
    sr^k = r^{-k}s, r^ks = sr^{-k}
  \]

  \centerline{$j_1$ even or odd?}
\end{frame}
%%%%%%%%%%%%%%%
\begin{frame}{(TJ 9.16)}
  \centerline{$f$ is one-to-one}

  \[
    f(r^{i_1}s^{j_1}) = f(r^{i_2}s^{j_2})
  \]

  \[
    \rho^{i_1}\lambda^{j_1} = \rho^{i_2}\lambda^{j_2},\; 1^{i_1 + j_1} = 1^{i_2 + j_2}
  \]

  \[
    \rho^{i_1 - i_2} = \lambda^{j_2 - j_1}
  \]

  \[
    i_1 = i_2,\; j_1 = j_2 
  \]
\end{frame}
%%%%%%%%%%%%%%%
\begin{frame}{(TJ 9.16)}
  \[
    H = \langle r^2, s \rangle \cong D_{n}
  \]

  \[
    Z = \set{1, r^n}
  \]

  \[
    D_{2n} = HZ,\quad H \cap Z = \emptyset,\quad hz = zh\; \forall h \in H, z \in Z
  \]

  \[
    G \cong H \times Z\quad (\textrm{Theorem 9.27, P158, 2016; Theorem 9.13, P150, 2010})
  \]

  \[
    |Z(D_{2n})| = 2,\; |Z(D_n \times \mathbb{Z}_{2})| = 4\quad (\textrm{if } n = 2k)
  \]
\end{frame}
%%%%%%%%%%%%%%%
\begin{frame}{(TJ 9.23)}
  \[
    G \times K \cong H \times K \centernot\implies G \cong H
  \]

  \[
    G = \mathbb{Z}, \quad H = {1}, \quad K = \prod_{n \in \mathbb{N}} \mathbb{Z}
  \]

  \centerline{``On Cancellation in Groups'' by R. Hirshon, 1969}

  \[
    G \times K \cong H \times K \quad \textcolor{red}{|K| < \infty} \implies G \cong H
  \]
\end{frame}
%%%%%%%%%%%%%%%
\begin{frame}{(TJ 11.18)}
  \begin{itemize}
    \item $\phi: G_1 \to G_2$
    \item $H_1 \triangleleft G_1$
    \item $\phi(H_1) = H_2$
    \item $G_1/H_1 \cong G_2/H_2$
  \end{itemize}

  \[
    G_1 = \mathbb{Z}_{2} \quad G_2 = \set{e} \quad H_1 = \set{0} \quad H_2 = \set{e}
  \]
\end{frame}
%%%%%%%%%%%%%%%
\begin{frame}{(TJ 11.5)}
  \[
    \phi: \mathbb{Z}_{24} \to \mathbb{Z}_{18}
  \]

  \begin{align*}
    \phi(1) = a & \implies \phi(x) = ax\; (\mathrm{mod} 18) \\
	    & \implies Ker(\phi) = \mathbb{Z}_{b} \cap \mathbb{Z}_{24}: ab \equiv 0\; (\mathrm{mod} 18)
  \end{align*}

  \[
    \phi(1) = ?
  \]

  \[
    |\phi(1)| | 18 \land |\phi(1)| | 24 \implies |\phi(1)| | 6
  \]

  \[
    \phi(1) = 0, 9, 6, 12, 3, 15
  \]

  \begin{align*}
    \phi_3(x) = 6x, \quad Ker(\phi_{3}) = 3\mathbb{Z}_{24}
  \end{align*}
\end{frame}
%%%%%%%%%%%%%%%
\begin{frame}{Normal subgroups}
  \[
    \mathbb{Z}/n\mathbb{Z}
  \]

  \[
    (aH) (bH) = (abH)
  \]

  \[
  \forall a, b \in G, \forall h_1, h_2 \in H, (ah_1) \in aH, (bh_2) \in bH: (ah_1)(bh_2) \in abH
  \]

  \[
    \exists h_3 \in H, (ah_1)(bh_2) = abh_3 \iff h_1 b = bh_3h_2^{-1}
  \]

  \[
    \forall b \in G, \forall h_1 \in H: \exists h' \in H: h_1 b = bh'
  \]

  \[
    \forall g \in G, \forall h \in H: \exists h' \in H: hg = gh'
  \]
\end{frame}
%%%%%%%%%%%%%%%
\begin{frame}{Normal subgroups}
  \[
    \forall g \in G, \forall h \in H: \exists h' \in H: hg = gh'
  \]

  \[
    \forall g \in G, Hg \subseteq gH
  \]

  \[
    \forall g^{-1} \in G, Hg^{-1} \subseteq g^{-1}H
  \]

  \[
    \forall h \in H, \exists h' \in H: hg^{-1} = g^{-1}h' \iff gh = h'g
  \]

  \[
    \forall g \in G,  Hg \subseteq gH
  \]

  \[
    \forall g \in G,  Hg = gH
  \]
\end{frame}
%%%%%%%%%%%%%%%
\begin{frame}{Normal subgroups}
  \[
    \forall g \in G, \forall h \in H: \exists h' \in H: hg = gh' \iff g^{-1}hg = h'
  \]

  \[
    \forall g \in G, g^{-1}Hg \subseteq H
  \]

  \[
    \forall g \in G, (g^{-1})^{-1}Hg^{-1} = gHg^{-1} \subseteq H
  \]

  \[
   \forall g \in G, \forall h \in H, \exists h' \in H: ghg^{-1} = h' \iff h = g^{-1}h'g
  \]

  \[
    \forall g \in G, H \subseteq g^{-1}Hg
  \]

  \[
    \forall g \in G, g^{-1}Hg = H
  \]

  \[
    \forall g \in G, gHg^{-1} = H
  \]
\end{frame}
%%%%%%%%%%%%%%%
\begin{frame}{(TJ 10.13)}
  \[
    g \in G, C(g) = \set{x \in G: gx = xg}
  \]

  \[
    Z(G) = \set{x \in G: gx = xg,  \forall g \in G} \implies Z(G) \triangleleft G
  \]

  \[
    C(g) \le G
  \]

  \[
    \langle g \rangle \triangleleft G \implies C(g) \triangleleft G
  \]
\end{frame}
%%%%%%%%%%%%%%%
\begin{frame}{(TJ 10.13)}
  \[
    \forall k \in G, x \in C(g): k^{-1} x k \in C(g)
  \]

  \[
    \forall k \in G, x \in C(g): gk^{-1}xk = k^{-1}xkg
  \]

  \[
    \langle g \rangle \triangleleft G \implies k \langle g \rangle = \langle g \rangle k \implies
    \exists t, kg = g^{t}k \iff gk^{-1} = k^{-1}g^t
  \]

  \[
    gk^{-1}xk = k^{-1}xg^{t}k \iff k^{-1}g^{t}xk = k^{-1}xg^{t}k
  \]
\end{frame}
%%%%%%%%%%%%%%%
